update tests, fix tutorial

tests/lean/Tutorial/Tutorial.lean
@@ -424,25 +424,16 @@ def add
 def dummy_hash (i : Std.U32) : Result Std.U32 := do
   ok 1000#u32
 
-/-- [tutorial::pseudo_random]: loop body 0:
-    Source: 'src/lib.rs', lines 258:2-260:3
-    Visibility: public -/
-@[rust_loop_body]
-def pseudo_random_loop.body
-  (state : Std.U32) : Result (ControlFlow Std.U32 Std.U32) := do
-  if state < 100#u32
-  then let state1 ← dummy_hash state
-       ok (cont state1)
-  else ok (done state)
-
 /-- [tutorial::pseudo_random]: loop 0:
     Source: 'src/lib.rs', lines 258:2-260:3
     Visibility: public -/
 @[rust_loop]
 def pseudo_random_loop (state : Std.U32) : Result Std.U32 := do
-  loop
-    (fun state1 => pseudo_random_loop.body state1)
-    state
+  if state < 100#u32
+  then let state1 ← dummy_hash state
+       pseudo_random_loop state1
+  else ok state
+partial_fixpoint
 
 /-- [tutorial::pseudo_random]:
     Source: 'src/lib.rs', lines 255:0-262:1
