tests/lean/Tutorial/Solutions.lean
@@ -456,17 +456,16 @@ theorem add_with_carry_spec
 theorem pseudo_random_spec :
   pseudo_random div⦃fun x => x.val >= 100⦄ := by
   unfold pseudo_random
-  unfold pseudo_random_loop
+  -- unfold pseudo_random_loop
   -- if we proceed by unfolding `loop`, then the proof will be non-terminating.
   -- instead, we can use the dspec_induction tactic
   -- note here that we must make a potentially non-obvious decision about
   -- what to generalize and how to do the induction
   generalize 0#u32 = x
   revert x
-  dspec_induction loop
+  dspec_induction pseudo_random_loop
   intros loop' ih x
   simp only
-  unfold pseudo_random_loop.body
   simp
   by_cases ((↑x : Nat) < 100)
   ·
